---
title: Geometric Progression and the Compounding of the Returns
description: Your savings account offers a 1% annual interest! The account balance in 10 years? +10%? Naaaah   
date: 2020-12-06T11:00:00.000Z
topic: mathematics
author: chris
img: /static/fractal-star.png
---

## Compounding of Returns

Let us consider the following scenario. A stock asset yields an average monthly return R of 2% for the last 12 months. If we had invested 100$ on this asset a year ago, what would be the outcome of this investment today?

Consider the initial asset price $P_0 = 100$. After the first month of the investment the outcome would be:

$$
P_1 = 100 + (100 * 0.02) = (100 * 1) + (100 * 0.02) = 100 * (1 + 0.02) = P_0 * 1.02
$$

The outcome after the 2nd month would be:

$$
P_2 = P_1 + (P_1 * 0.02) = P_1 * 1.02
$$

3rd month:

$$
P_3 = P_2 + (P_2 * 0.02) = P_2 * 1.02
$$

(ν-1)th month:

$$
P_(ν-1) = P_(ν-2) + (P_(ν-2) * 0.02) = P_(ν-2) * 1.02
$$

νth month:

$$
P_ν = P_(ν-1) + (P_(ν-1) * 0.02) = P_(ν-1) * 1.02
$$

It becomes obvious from the above that generating each element in the sequence $P_0, P_1, ..., P_(ν-1), P_ν$ follows a pattern where the present number is generated by multiplying the previous number with a constant.

In our case, the constant is the average monthly return + 1. If we combine the previous equations in an attempt to formulate a final equation that provides the νth based on the $P_0$ element then:

$$
P_ν = P_(ν-1) * 1.02 = (P_(ν-2) * 1.02) * 1.02 = P_(ν-2) * 1.02^2 = .... = P_0 * (1 + 0.02)^ν
$$

So, after 12 months we will have $100 * 1.02^12 = 126.82$!

The generic equation is:

$$
P_ν = P_0 * (1 + R_ν)^ν \qquad (1)
$$

## Geometric Progression

In calculus, a sequence of numbers where each term after the first is found by multiplying the previous one by a fixed, non-one number, called `geometric progression`. The fixed number is called, the `common ratio`.

Some interesting properties to notice:

* a common ratio greater than 1, will produce exponential growth towards positive infinity!
* a common ratio greater than 0 and up to 1, will produce exponential decay towards zero!

In the example above the way we used the return to calculate the end result is called **Compounding of Returns**.

## From annual to periodic returns

Let's see the example above from another angle. Let's say that an assets had a total return over the last year of 10%. What was the average monthly return of the asset?

We calculate a simple/arithmetic return (pandas.pct_change) like:

$$
R_i = \frac{P_i-P_{i-1}}{P_{i-1}} = \frac{P_i}{P_{i-1}} - 1 \qquad (2)
$$

where $P_i$ is the price of the asset on the period $i$.

By assuming (for simplicity) that $P_0 = 1$ and from (2), $P_1 = P_0 * (1 + R_{annual})$

Then from (1),

$$
1 + R_{annual} = 1 * (1 + R_{month})^12 => R_{month} = \sqrt[12]{1+R_{annual}} - 1 (3)
$$

We use ν = 12, because 1 year = 12 months (=> 12 compounding periods). If instead of monthly returns we were asked to find quarter returns then we would use ν = 4 ($R_{quarter} = \sqrt[4]{1+R_{annual}} - 1$).

Finally, from (3),

$$
R_{monthly} = \sqrt[12]{1 + 0.1} - 1 = \sqrt[12]{1.1} - 1 = 1.0079 - 1 = 0.0079
$$

## Compounding variable returns

It is commonly accepted that returns do not stay the same over periods. For example, the average return of this month is not the same as the one from last month! However, the same principle of compounding applies in this case too. Let's see an example.

An asset yields the following return for the past couple of months $0.021, 0.032, -0.018, 0.06, -0.043, 0.048$. The total return is the **product** of the individual returns when 1 is added to them:

$$
R = (1 + 0.021) * (1 + 0.032) * (1 - 0.018) * (1 + 0.06) * (1 - 0.043) * (1 + 0.048) = ...
$$

This, resonates with the equation (1) above where for a fixed return we have $R_{total} = (1 + R_{fixed})^{number-of-periods}$